Backport endianness lemmas from HACL*. Implement `upd_32_be`

kremlib/C.Endianness.fst
@@ -196,3 +196,60 @@ let index_64_le (b: B.buffer UInt8.t) (i: UInt32.t):
       r = Seq.index (seq_uint64_of_le (B.length b / 8) (B.as_seq h0 b)) (UInt32.v i)))
 =
   load64_le (B.sub b FStar.UInt32.(8ul *^ i) 8ul)
+
+#reset-options "--using_facts_from '* -FStar.UInt8 -FStar.UInt16 -FStar.UInt32 -FStar.UInt64 -FStar.Int8 -FStar.Int16 -FStar.Int32 -FStar.Int64'"
+
+let interval_4_disjoint (i j: nat) : Lemma
+  (requires (i <> j))
+  (ensures (let open FStar.Mul in 4 * i + 4 <= 4 * j \/ 4 * j + 4 <= 4 * i))
+= ()
+
+#reset-options "--z3rlimit 16"
+
+let upd_32_be (b: B.buffer UInt8.t) (i: UInt32.t) (v: UInt32.t):
+  Stack unit
+    (requires (fun h ->
+      B.live h b /\ B.length b % 4 = 0 /\
+      UInt32.v i < B.length b / 4))
+    (ensures (fun h0 _ h1 ->
+      B.(modifies (loc_buffer b) h0 h1) /\
+      seq_uint32_of_be (B.length b / 4) (B.as_seq h1 b) `Seq.equal` Seq.upd (seq_uint32_of_be (B.length b / 4) (B.as_seq h0 b)) (UInt32.v i) v
+    ))
+= let h0 = get () in
+  store32_be (B.sub b FStar.UInt32.(4ul *^ i) 4ul) v;
+  let h1 = get () in
+  let f () : Lemma
+    (seq_uint32_of_be (B.length b / 4) (B.as_seq h1 b) `Seq.equal` Seq.upd (seq_uint32_of_be (B.length b / 4) (B.as_seq h0 b)) (UInt32.v i) v)
+  = let s0 = B.as_seq h0 b in
+    let s1 = B.as_seq h1 b in
+    let n = B.length b / 4 in
+    assert (4 `Prims.op_Multiply` n == B.length b);
+    let s0' = seq_uint32_of_be n s0 in
+    let s1' = seq_uint32_of_be n s1 in
+    let lo = UInt32.v i in
+    let hi = lo + 1 in
+    let s2' = Seq.upd s0' lo v in
+    assert (Seq.length s1' == Seq.length s2');
+    let f
+      (j: nat)
+    : Lemma
+      (requires (j < n))
+      (ensures (j < n /\ Seq.index s1' j == Seq.index s2' j))
+    =
+      if j = lo
+      then ()
+      else begin
+        slice_seq_uint32_of_be n s0 j (j + 1);
+        slice_seq_uint32_of_be n s1 j (j + 1);
+        let bj = B.gsub b (4ul `UInt32.mul` UInt32.uint_to_t j) 4ul in
+        let sj0 = seq_uint32_of_be 1 (B.as_seq h0 bj) in
+        let sj1 = seq_uint32_of_be 1 (B.as_seq h1 bj) in
+        assert (Seq.index s1' j == Seq.index sj1 0);
+        assert (Seq.index s0' j == Seq.index sj0 0);
+        interval_4_disjoint j lo;
+        ()
+      end
+    in
+    Classical.forall_intro (Classical.move_requires f)
+  in
+  f ()
